copy word cleanup, todos

theories/examples/copy_word.v
@@ -15,11 +15,10 @@ Section copy_word.
   Definition program' (instr: list Word) (b:Addr):=
     ([∗ list] a;w ∈ (finz.seq b (length instr));instr, (a ->a w))%I.
   
-  Lemma copy_word {p prx progpage srcpage dstpage sacc i q qi w w_ r0_ r1_} src dst :
-    p ≠ srcpage ->
+  Lemma copy_word {ptx prx progpage srcpage dstpage sacc i q qi w w_ r0_ r1_} src dst :
+    ptx ≠ srcpage ->
     prx ≠ dstpage ->
     seq_in_page (of_pid progpage) (length (program src dst)) progpage ->
-    to_pid_aligned src ≠ p ->
     not (addr_in_page src progpage) ->
     not (addr_in_page dst progpage) ->
     addr_in_page src srcpage ->
@@ -34,7 +33,7 @@ Section copy_word.
     ∗ (dst ->a w_)
     ∗ (R0 @@ i ->r r0_)
     ∗ (R1 @@ i ->r r1_)
-    ∗ (TX@ i := p)
+    ∗ (TX@ i := ptx)
     ∗ (<<i>>{ qi })
     ∗ (RX@ i := prx)
     ⊢ (PARWP ExecI @ i
@@ -48,9 +47,9 @@ Section copy_word.
           ∗ R1 @@ i ->r w
           ∗ (<<i>>{ qi })
           ∗ (RX@ i := prx)
-          ∗ (TX@ i := p))}}%I).
+          ∗ (TX@ i := ptx))}}%I).
   Proof.
-    iIntros (Hneq Hneq''' Hseqp Hal Hneq' Hneq'' Hsrcp Hdstp Hprpain Hsrcpain Hdstpain) "(Hbstar & Hai & Hpc & Hsrc & Hdst & Hr0 & Hr1 & HTX & Hi & HRX)".
+    iIntros (Hneq Hneq' Hseqp Hnin Hnin' Hsrcp Hdstp Hprpain Hsrcpain Hdstpain) "(Hbstar & Hai & Hpc & Hsrc & Hdst & Hr0 & Hr1 & HTX & Hi & HRX)".
     apply seq_in_page_forall in Hseqp.
     rewrite <-parwp_sswp.
     iDestruct "Hbstar" as "(p_start & Hbstar)".
@@ -70,7 +69,7 @@ Section copy_word.
           rewrite ->Forall_forall in Hseqp.
           specialize (Hseqp (progpage ^+ 1)%f).
           rewrite C in Hseqp.
-          apply Hneq'.
+          apply Hnin.
           apply Hseqp.
           rewrite <-C.
           rewrite finz_seq_cons.
@@ -83,19 +82,23 @@ Section copy_word.
     reflexivity.
     instantiate (1 := encode_instruction (Ldr R1 R0)).
     by rewrite decode_encode_instruction.
-    instantiate (1 := p).
-    assumption.
+    instantiate (1 := ptx).
+    intros C.
+    apply to_pid_aligned_in_page in Hsrcp.
+    rewrite <-Hsrcp in Hneq.
+    rewrite C in Hneq.
+    apply Hneq.
+    reflexivity.
+    rewrite ->Forall_forall in Hseqp.
+    specialize (Hseqp (progpage ^+ 1)%f).
     instantiate (1 := sacc).
     apply to_pid_aligned_in_page in Hsrcp.
     subst srcpage.
-    rewrite ->Forall_forall in Hseqp.
-    specialize (Hseqp (progpage ^+ 1)%f).
-    pose proof (to_pid_aligned_in_page (progpage ^+ 1)%f progpage).
-    assert ((progpage ^+ 1)%f ∈ finz.seq progpage (length (program src dst))).
+    assert (Hp : (progpage ^+ 1)%f ∈ finz.seq progpage (length (program src dst))).
     set_solver.
-    pose proof (Hseqp H1).
-    pose proof (H0 H2).
-    rewrite H3.
+    specialize (Hseqp Hp).
+    apply to_pid_aligned_in_page in Hseqp.
+    rewrite Hseqp.
     set_solver.
     iFrame.
     iApply "J".
@@ -123,7 +126,7 @@ Section copy_word.
     rewrite ->Forall_forall in Hseqp.
     specialize (Hseqp (((progpage ^+ 1) ^+ 1) ^+ 1)%f).
     rewrite C in Hseqp.
-    apply Hneq''.
+    apply Hnin'.
     apply Hseqp.
     rewrite <-C.
     rewrite finz_seq_cons.
@@ -133,8 +136,8 @@ Section copy_word.
     lia.
     instantiate (1 := prx).
     intros C.
-    rewrite C in Hneq'''.
-    apply Hneq'''.
+    rewrite C in Hneq'.
+    apply Hneq'.
     apply to_pid_aligned_in_page in Hdstp.
     assumption.
     instantiate (1 := sacc).
@@ -142,12 +145,12 @@ Section copy_word.
     subst dstpage.
     rewrite ->Forall_forall in Hseqp.
     specialize (Hseqp (((progpage ^+ 1) ^+ 1) ^+ 1)%f).
-    pose proof (to_pid_aligned_in_page (((progpage ^+ 1) ^+ 1) ^+ 1)%f progpage).
-    assert ((((progpage ^+ 1) ^+ 1) ^+ 1)%f ∈ finz.seq progpage (length (program src dst))).
+    pose proof (to_pid_aligned_in_page (((progpage ^+ 1) ^+ 1) ^+ 1)%f progpage) as Hp.
+    assert (Hq : (((progpage ^+ 1) ^+ 1) ^+ 1)%f ∈ finz.seq progpage (length (program src dst))).
     set_solver.
-    pose proof (Hseqp H1).
-    pose proof (H0 H2).
-    rewrite H3.
+    specialize (Hseqp Hq).
+    specialize (Hp Hseqp).
+    rewrite Hp.
     set_solver.
     iFrame.
     iApply "J".
@@ -156,12 +159,93 @@ Section copy_word.
     iApply parwp_finish.
     iFrame.
     iSplit; auto.
-    assert ((progpage ^+ length (program src dst))%f = ((((progpage ^+ 1) ^+ 1) ^+ 1) ^+ 1)%f).
-    assert (Z.of_nat (length (program src dst)) = 4%Z). by compute.
-    rewrite H0.
+    assert (Hp : (progpage ^+ length (program src dst))%f = ((((progpage ^+ 1) ^+ 1) ^+ 1) ^+ 1)%f).
+    assert (Hq : Z.of_nat (length (program src dst)) = 4%Z). by compute.
+    rewrite Hq.
     solve_finz.
-    rewrite H0.
+    rewrite Hp.
     iFrame.
   Qed.
+
+  (* TODOs:
+     - sub and add
+     - loop rule ???
+     - branch rule ???
+   *)
+  (*
+  Definition cmp_I ra := encode_instruction (Cmp ra).
+  Definition bne_I ra := encode_instruction (Bne ra).
+  Definition sub_word_I ra w := encode_instruction (Sub ra (inl w)).
+  Definition add_word_I ra w := encode_instruction (Add ra (inl w)).
+  Definition sub_reg_I ra rb := encode_instruction (Sub ra (inr rb)).
+  Definition add_reg_I ra rb := encode_instruction (Add ra (inr rb)).
+  Definition mov_reg_I ra rb := encode_instruction (Mov ra (inr rb)).
   
+  Definition program_c step src dst :=
+    [
+    mov_word_I R2 step; (* remaining runs *)
+    mov_word_I R4 0;    (* counter *)
+    mov_reg_I R3 PC;    (* program base address *)
+    add_I R3 2;         (* loop base address *)
+    (* loop body begin *)
+    (* loop may depend on step and counter
+       it should restore PC, R2, R4
+       perhaps, we could try to write a special rule for loops
+     *)
+    (* ldr data from src + counter to R1 *)
+    mov_word_I R0 src;
+    add_I R0 R4;
+    ldr_I R1 R0;
+    (* str data from R1 to dst + counter *)
+    mov_word_I R0 dst;
+    add_I R0 R4;
+    str_I R1 R0;
+    (* loop body end *)
+    (* incr counter *)
+    add_I R4 1;
+    (* decr remaining runs *)
+    sub_I R2 1;
+    (* conditional jump *)
+    (* might be a good idea to have a separate rule for branches *)
+    cmp_I R2;
+    bne_I R3
+    ].
+  
+  Lemma copy_words {ptx prx progpage srcpage dstpage sacc i q qi w w_ r0_ r1_} step src dst :
+    step < page_size ->
+    length mem = step ->
+    ptx ≠ srcpage ->
+    prx ≠ dstpage ->
+    seq_in_page (of_pid progpage) (length (program_c step src dst)) progpage ->
+    not (addr_in_page src progpage) ->
+    not (addr_in_page dst progpage) ->
+    addr_in_page src srcpage ->
+    addr_in_page dst dstpage ->
+    progpage ∈ sacc ->
+    srcpage ∈ sacc ->
+    dstpage ∈ sacc ->
+    program' (program_c step src dst) (of_pid progpage)
+    ∗ A@i :={q}[sacc]
+    ∗ PC @@ i ->r (of_pid progpage)
+    ∗ mem_region mem srcpage
+    ∗ (∃ m, mem_region m dstpage)
+    ∗ (R0 @@ i ->r r0_)
+    ∗ (R1 @@ i ->r r1_)
+    ∗ (TX@ i := ptx)
+    ∗ (<<i>>{ qi })
+    ∗ (RX@ i := prx)
+    ⊢ (PARWP ExecI @ i
+          {{ (λ m, ⌜m = ExecI⌝
+          ∗ program' (program_c step src dst) (of_pid progpage)
+          ∗ A@i :={q}[sacc]
+          ∗ PC @@ i ->r ((of_pid progpage) ^+ (length (program src dst)))%f
+          ∗ mem_region mem srcpage
+          ∗ mem_region mem dstpage
+          ∗ R0 @@ i ->r dst
+          ∗ R1 @@ i ->r w
+          ∗ (<<i>>{ qi })
+          ∗ (RX@ i := prx)
+          ∗ (TX@ i := ptx))}}%I).
+  Admitted.
+  *)
 End copy_word.
